cedar-lean/Cedar/Thm/Validation/Slice/Reachable/IfThenElse.lean
@@ -30,7 +30,7 @@ open Cedar.Data
 open Cedar.Spec
 open Cedar.Validation
 
-theorem checked_eval_entity_reachable_ite {e₁ e₂ e₃: Expr} {n : Nat} {c c' : Capabilities} {tx : TypedExpr} {env : Environment} {entities : Entities} {path : List Attr}
+theorem checked_eval_entity_reachable_ite {e₁ e₂ e₃: Expr} {n : Nat} {c c' : Capabilities} {tx : TypedExpr} {env : TypeEnv} {entities : Entities} {path : List Attr}
   (hc : CapabilitiesInvariant c request entities)
   (hr : InstanceOfWellFormedEnvironment request entities env)
   (ht : typeOf (.ite e₁ e₂ e₃) c env = .ok (tx, c'))
