cedar-lean/Cedar/Thm/Validation/Typechecker/BinaryApp/ContainsAnyAll.lean
@@ -26,7 +26,7 @@ open Cedar.Data
 open Cedar.Spec
 open Cedar.Validation
 
-theorem type_of_containsA_inversion {op₂ : BinaryOp} {x₁ x₂ : Expr} {c c' : Capabilities} {env : Environment} {ty : TypedExpr}
+theorem type_of_containsA_inversion {op₂ : BinaryOp} {x₁ x₂ : Expr} {c c' : Capabilities} {env : TypeEnv} {ty : TypedExpr}
   (h₁ : op₂ = .containsAll ∨ op₂ = .containsAny)
   (h₂ : typeOf (Expr.binaryApp op₂ x₁ x₂) c env = Except.ok (ty, c')) :
   c' = ∅ ∧
@@ -56,7 +56,7 @@ theorem type_of_containsA_inversion {op₂ : BinaryOp} {x₁ x₂ : Expr} {c c' 
   }
 
 
-theorem type_of_containsA_is_sound {op₂ : BinaryOp} {x₁ x₂ : Expr} {c₁ c₂ : Capabilities} {env : Environment} {ty : TypedExpr} {request : Request} {entities : Entities}
+theorem type_of_containsA_is_sound {op₂ : BinaryOp} {x₁ x₂ : Expr} {c₁ c₂ : Capabilities} {env : TypeEnv} {ty : TypedExpr} {request : Request} {entities : Entities}
   (h₀ : op₂ = .containsAll ∨ op₂ = .containsAny)
   (h₁ : CapabilitiesInvariant c₁ request entities)
   (h₂ : InstanceOfWellFormedEnvironment request entities env)
