cedar-lean/Cedar/Thm/Validation/Typechecker/Call.lean
@@ -26,7 +26,7 @@ open Cedar.Data
 open Cedar.Spec
 open Cedar.Validation
 
-theorem type_of_call_args_inversion {xs : List Expr} {txs : List TypedExpr} {c : Capabilities} {env : Environment}
+theorem type_of_call_args_inversion {xs : List Expr} {txs : List TypedExpr} {c : Capabilities} {env : TypeEnv}
   (htxs : (xs.mapM₁ λ x => justType (typeOf x.val c env)) = Except.ok txs) :
   List.Forall₂ (λ xᵢ txᵢ => ∃ cᵢ, typeOf xᵢ c env = Except.ok (txᵢ, cᵢ)) xs txs
 :=
@@ -52,7 +52,7 @@ match xs with
   · have ih := @type_of_call_args_inversion xs
     simp [ih, htxs', List.mapM₁]
 
-theorem type_of_call_inversion {xs : List Expr} {c c' : Capabilities} {env : Environment} {tx : TypedExpr}
+theorem type_of_call_inversion {xs : List Expr} {c c' : Capabilities} {env : TypeEnv} {tx : TypedExpr}
   (htx : typeOf (Expr.call xfn xs) c env = Except.ok (tx, c')) :
   ∃ txs,
     (∃ ty, tx = .call xfn txs ty) ∧
@@ -75,7 +75,7 @@ theorem type_of_call_inversion {xs : List Expr} {c c' : Capabilities} {env : Env
     simp [←htx]
   · exact type_of_call_args_inversion htx₁
 
-theorem type_of_call_decimal_inversion {xs : List Expr} {c c' : Capabilities} {env : Environment} {ty : TypedExpr}
+theorem type_of_call_decimal_inversion {xs : List Expr} {c c' : Capabilities} {env : TypeEnv} {ty : TypedExpr}
   (h₁ : typeOf (Expr.call .decimal xs) c env = Except.ok (ty, c')) :
   ty.typeOf = .ext .decimal ∧
   c' = ∅ ∧
@@ -95,7 +95,7 @@ theorem type_of_call_decimal_inversion {xs : List Expr} {c c' : Capabilities} {e
   rename_i h₃
   simp [TypedExpr.typeOf, h₃]
 
-theorem type_of_call_decimal_is_sound {xs : List Expr} {c₁ c₂ : Capabilities} {env : Environment} {ty : TypedExpr} {request : Request} {entities : Entities}
+theorem type_of_call_decimal_is_sound {xs : List Expr} {c₁ c₂ : Capabilities} {env : TypeEnv} {ty : TypedExpr} {request : Request} {entities : Entities}
   (h₁ : typeOf (Expr.call .decimal xs) c₁ env = Except.ok (ty, c₂)) :
   GuardedCapabilitiesInvariant (Expr.call .decimal xs) c₂ request entities ∧
   ∃ v, EvaluatesTo (Expr.call .decimal xs) request entities v ∧ InstanceOfType env v ty.typeOf
@@ -112,7 +112,7 @@ theorem type_of_call_decimal_is_sound {xs : List Expr} {c₁ c₂ : Capabilities
   · apply InstanceOfType.instance_of_ext
     simp [InstanceOfExtType]
 
-theorem type_of_call_datetime_inversion {xs : List Expr} {c c' : Capabilities} {env : Environment} {ty : TypedExpr}
+theorem type_of_call_datetime_inversion {xs : List Expr} {c c' : Capabilities} {env : TypeEnv} {ty : TypedExpr}
   (h₁ : typeOf (Expr.call .datetime xs) c env = Except.ok (ty, c')) :
   ty.typeOf = .ext .datetime ∧
   c' = ∅ ∧
@@ -134,7 +134,7 @@ theorem type_of_call_datetime_inversion {xs : List Expr} {c c' : Capabilities} {
   cases h₁ ; subst ty
   simp only [TypedExpr.typeOf, h₃, Option.isSome_some, and_self]
 
-theorem type_of_call_datetime_is_sound {xs : List Expr} {c₁ c₂ : Capabilities} {env : Environment} {ty : TypedExpr} {request : Request} {entities : Entities}
+theorem type_of_call_datetime_is_sound {xs : List Expr} {c₁ c₂ : Capabilities} {env : TypeEnv} {ty : TypedExpr} {request : Request} {entities : Entities}
   (h₁ : typeOf (Expr.call .datetime xs) c₁ env = Except.ok (ty, c₂)) :
   GuardedCapabilitiesInvariant (Expr.call .datetime xs) c₂ request entities ∧
   ∃ v, EvaluatesTo (Expr.call .datetime xs) request entities v ∧ InstanceOfType env v ty.typeOf
@@ -151,7 +151,7 @@ theorem type_of_call_datetime_is_sound {xs : List Expr} {c₁ c₂ : Capabilitie
   · apply InstanceOfType.instance_of_ext
     simp [InstanceOfExtType]
 
-theorem type_of_call_duration_inversion {xs : List Expr} {c c' : Capabilities} {env : Environment} {ty : TypedExpr}
+theorem type_of_call_duration_inversion {xs : List Expr} {c c' : Capabilities} {env : TypeEnv} {ty : TypedExpr}
   (h₁ : typeOf (Expr.call .duration xs) c env = Except.ok (ty, c')) :
   ty.typeOf = .ext .duration ∧
   c' = ∅ ∧
@@ -171,7 +171,7 @@ theorem type_of_call_duration_inversion {xs : List Expr} {c c' : Capabilities} {
   rename_i h₃
   simp [TypedExpr.typeOf, h₃]
 
-theorem type_of_call_duration_is_sound {xs : List Expr} {c₁ c₂ : Capabilities} {env : Environment} {ty : TypedExpr} {request : Request} {entities : Entities}
+theorem type_of_call_duration_is_sound {xs : List Expr} {c₁ c₂ : Capabilities} {env : TypeEnv} {ty : TypedExpr} {request : Request} {entities : Entities}
   (h₁ : typeOf (Expr.call .duration xs) c₁ env = Except.ok (ty, c₂)) :
   GuardedCapabilitiesInvariant (Expr.call .duration xs) c₂ request entities ∧
   ∃ v, EvaluatesTo (Expr.call .duration xs) request entities v ∧ InstanceOfType env v ty.typeOf
@@ -188,7 +188,7 @@ theorem type_of_call_duration_is_sound {xs : List Expr} {c₁ c₂ : Capabilitie
   · apply InstanceOfType.instance_of_ext
     simp [InstanceOfExtType]
 
-theorem type_of_call_ip_inversion {xs : List Expr} {c c' : Capabilities} {env : Environment} {ty : TypedExpr}
+theorem type_of_call_ip_inversion {xs : List Expr} {c c' : Capabilities} {env : TypeEnv} {ty : TypedExpr}
   (h₁ : typeOf (Expr.call .ip xs) c env = Except.ok (ty, c')) :
   ty.typeOf = .ext .ipAddr ∧
   c' = ∅ ∧
@@ -209,7 +209,7 @@ theorem type_of_call_ip_inversion {xs : List Expr} {c c' : Capabilities} {env : 
   cases h₁ ; subst ty
   simp [h₃, TypedExpr.typeOf]
 
-theorem type_of_call_ip_is_sound {xs : List Expr} {c₁ c₂ : Capabilities} {env : Environment} {ty : TypedExpr} {request : Request} {entities : Entities}
+theorem type_of_call_ip_is_sound {xs : List Expr} {c₁ c₂ : Capabilities} {env : TypeEnv} {ty : TypedExpr} {request : Request} {entities : Entities}
   (h₁ : typeOf (Expr.call .ip xs) c₁ env = Except.ok (ty, c₂)) :
   GuardedCapabilitiesInvariant (Expr.call .ip xs) c₂ request entities ∧
   ∃ v, EvaluatesTo (Expr.call .ip xs) request entities v ∧ InstanceOfType env v ty.typeOf
@@ -226,7 +226,7 @@ theorem type_of_call_ip_is_sound {xs : List Expr} {c₁ c₂ : Capabilities} {en
   · apply InstanceOfType.instance_of_ext
     simp [InstanceOfExtType]
 
-theorem typeOf_of_binary_call_inversion {xs : List Expr} {c : Capabilities} {env : Environment} {ty₁ ty₂ : TypedExpr}
+theorem typeOf_of_binary_call_inversion {xs : List Expr} {c : Capabilities} {env : TypeEnv} {ty₁ ty₂ : TypedExpr}
   (h₁ : (xs.mapM₁ fun x => justType (typeOf x.val c env)) = Except.ok [ty₁, ty₂]) :
   ∃ x₁ x₂ c₁ c₂,
     xs = [x₁, x₂] ∧
@@ -278,7 +278,7 @@ def IsDecimalComparator : ExtFun → Prop
   | .greaterThanOrEqual => True
   | _                   => False
 
-theorem type_of_call_decimal_comparator_inversion {xfn : ExtFun} {xs : List Expr} {c c' : Capabilities} {env : Environment} {ty : TypedExpr}
+theorem type_of_call_decimal_comparator_inversion {xfn : ExtFun} {xs : List Expr} {c c' : Capabilities} {env : TypeEnv} {ty : TypedExpr}
   (h₀ : IsDecimalComparator xfn)
   (h₁ : typeOf (Expr.call xfn xs) c env = Except.ok (ty, c')) :
   ty.typeOf = .bool .anyBool ∧
@@ -315,7 +315,7 @@ theorem type_of_call_decimal_comparator_inversion {xfn : ExtFun} {xs : List Expr
     }
   }
 
-theorem type_of_call_decimal_comparator_is_sound {xfn : ExtFun} {xs : List Expr} {c₁ c₂ : Capabilities} {env : Environment} {ty : TypedExpr} {request : Request} {entities : Entities}
+theorem type_of_call_decimal_comparator_is_sound {xfn : ExtFun} {xs : List Expr} {c₁ c₂ : Capabilities} {env : TypeEnv} {ty : TypedExpr} {request : Request} {entities : Entities}
   (h₀ : IsDecimalComparator xfn)
   (h₁ : CapabilitiesInvariant c₁ request entities)
   (h₂ : InstanceOfWellFormedEnvironment request entities env)
@@ -357,7 +357,7 @@ theorem type_of_call_decimal_comparator_is_sound {xfn : ExtFun} {xs : List Expr}
   }
 
 
-theorem type_of_call_isInRange_inversion {xs : List Expr} {c c' : Capabilities} {env : Environment} {ty : TypedExpr}
+theorem type_of_call_isInRange_inversion {xs : List Expr} {c c' : Capabilities} {env : TypeEnv} {ty : TypedExpr}
   (h₁ : typeOf (Expr.call .isInRange xs) c env = Except.ok (ty, c')) :
   ty.typeOf = .bool .anyBool ∧
   c' = ∅ ∧
@@ -389,7 +389,7 @@ theorem type_of_call_isInRange_inversion {xs : List Expr} {c c' : Capabilities} 
     apply typeOf_of_binary_call_inversion h₂
   }
 
-theorem type_of_call_isInRange_comparator_is_sound {xs : List Expr} {c₁ c₂ : Capabilities} {env : Environment} {ty : TypedExpr} {request : Request} {entities : Entities}
+theorem type_of_call_isInRange_comparator_is_sound {xs : List Expr} {c₁ c₂ : Capabilities} {env : TypeEnv} {ty : TypedExpr} {request : Request} {entities : Entities}
   (h₁ : CapabilitiesInvariant c₁ request entities)
   (h₂ : InstanceOfWellFormedEnvironment request entities env)
   (h₃ : typeOf (Expr.call .isInRange xs) c₁ env = Except.ok (ty, c₂))
@@ -433,7 +433,7 @@ def IsIpAddrRecognizer : ExtFun → Prop
   | _            => False
 
 
-theorem typeOf_of_unary_call_inversion {xs : List Expr} {c : Capabilities} {env : Environment} {ty₁ : TypedExpr}
+theorem typeOf_of_unary_call_inversion {xs : List Expr} {c : Capabilities} {env : TypeEnv} {ty₁ : TypedExpr}
   (h₁ : (xs.mapM₁ fun x => justType (typeOf x.val c env)) = Except.ok [ty₁]) :
   ∃ x₁ c₁,
     xs = [x₁] ∧
@@ -468,7 +468,7 @@ theorem typeOf_of_unary_call_inversion {xs : List Expr} {c : Capabilities} {env 
       rename_i res₁ _ _ res₂ _
       cases h₂ : List.mapM (fun x => justType (typeOf x c env)) tl₂ <;> simp [h₂] at h₁
 
-theorem type_of_call_toTime_inversion {xs : List Expr} {c c' : Capabilities} {env : Environment} {ty : TypedExpr}
+theorem type_of_call_toTime_inversion {xs : List Expr} {c c' : Capabilities} {env : TypeEnv} {ty : TypedExpr}
   (h₁ : typeOf (Expr.call .toTime xs) c env = Except.ok (ty, c')) :
   ty.typeOf = .ext .duration ∧
   c' = ∅ ∧
@@ -497,7 +497,7 @@ theorem type_of_call_toTime_inversion {xs : List Expr} {c c' : Capabilities} {en
     }
   }
 
-theorem type_of_call_toTime_is_sound {xs : List Expr} {c₁ c₂ : Capabilities} {env : Environment} {ty : TypedExpr} {request : Request} {entities : Entities}
+theorem type_of_call_toTime_is_sound {xs : List Expr} {c₁ c₂ : Capabilities} {env : TypeEnv} {ty : TypedExpr} {request : Request} {entities : Entities}
   (h₁ : CapabilitiesInvariant c₁ request entities)
   (h₂ : InstanceOfWellFormedEnvironment request entities env)
   (h₃ : typeOf (Expr.call .toTime xs) c₁ env = Except.ok (ty, c₂))
@@ -528,7 +528,7 @@ theorem type_of_call_toTime_is_sound {xs : List Expr} {c₁ c₂ : Capabilities}
   apply InstanceOfType.instance_of_ext
   simp only [InstanceOfExtType]
 
-theorem type_of_call_toDate_inversion {xs : List Expr} {c c' : Capabilities} {env : Environment} {ty : TypedExpr}
+theorem type_of_call_toDate_inversion {xs : List Expr} {c c' : Capabilities} {env : TypeEnv} {ty : TypedExpr}
   (h₁ : typeOf (Expr.call .toDate xs) c env = Except.ok (ty, c')) :
   ty.typeOf = .ext .datetime ∧
   c' = ∅ ∧
@@ -557,7 +557,7 @@ theorem type_of_call_toDate_inversion {xs : List Expr} {c c' : Capabilities} {en
     }
   }
 
-theorem type_of_call_toDate_is_sound {xs : List Expr} {c₁ c₂ : Capabilities} {env : Environment} {ty : TypedExpr} {request : Request} {entities : Entities}
+theorem type_of_call_toDate_is_sound {xs : List Expr} {c₁ c₂ : Capabilities} {env : TypeEnv} {ty : TypedExpr} {request : Request} {entities : Entities}
   (h₁ : CapabilitiesInvariant c₁ request entities)
   (h₂ : InstanceOfWellFormedEnvironment request entities env)
   (h₃ : typeOf (Expr.call .toDate xs) c₁ env = Except.ok (ty, c₂))
@@ -593,7 +593,7 @@ theorem type_of_call_toDate_is_sound {xs : List Expr} {c₁ c₂ : Capabilities}
     simp only [Except.error.injEq, reduceCtorEq, or_self, or_false, or_true, true_and]
     apply type_is_inhabited_ext
 
-theorem type_of_call_offset_inversion {xs : List Expr} {c c' : Capabilities} {env : Environment} {ty : TypedExpr}
+theorem type_of_call_offset_inversion {xs : List Expr} {c c' : Capabilities} {env : TypeEnv} {ty : TypedExpr}
   (h₁ : typeOf (Expr.call .offset xs) c env = Except.ok (ty, c')) :
   ty.typeOf = .ext .datetime ∧
   c' = ∅ ∧
@@ -627,7 +627,7 @@ theorem type_of_call_offset_inversion {xs : List Expr} {c c' : Capabilities} {en
     }
   }
 
-theorem type_of_call_offset_is_sound {xs : List Expr} {c₁ c₂ : Capabilities} {env : Environment} {ty : TypedExpr} {request : Request} {entities : Entities}
+theorem type_of_call_offset_is_sound {xs : List Expr} {c₁ c₂ : Capabilities} {env : TypeEnv} {ty : TypedExpr} {request : Request} {entities : Entities}
   (h₁ : CapabilitiesInvariant c₁ request entities)
   (h₂ : InstanceOfWellFormedEnvironment request entities env)
   (h₃ : typeOf (Expr.call .offset xs) c₁ env = Except.ok (ty, c₂))
@@ -674,7 +674,7 @@ theorem type_of_call_offset_is_sound {xs : List Expr} {c₁ c₂ : Capabilities}
       simp only [Except.error.injEq, reduceCtorEq, or_self, or_false, or_true, true_and]
       apply type_is_inhabited_ext
 
-theorem type_of_call_durationSince_inversion {xs : List Expr} {c c' : Capabilities} {env : Environment} {ty : TypedExpr}
+theorem type_of_call_durationSince_inversion {xs : List Expr} {c c' : Capabilities} {env : TypeEnv} {ty : TypedExpr}
   (h₁ : typeOf (Expr.call .durationSince xs) c env = Except.ok (ty, c')) :
   ty.typeOf = .ext .duration ∧
   c' = ∅ ∧
@@ -708,7 +708,7 @@ theorem type_of_call_durationSince_inversion {xs : List Expr} {c c' : Capabiliti
     }
   }
 
-theorem type_of_call_durationSince_is_sound {xs : List Expr} {c₁ c₂ : Capabilities} {env : Environment} {ty : TypedExpr} {request : Request} {entities : Entities}
+theorem type_of_call_durationSince_is_sound {xs : List Expr} {c₁ c₂ : Capabilities} {env : TypeEnv} {ty : TypedExpr} {request : Request} {entities : Entities}
   (h₁ : CapabilitiesInvariant c₁ request entities)
   (h₂ : InstanceOfWellFormedEnvironment request entities env)
   (h₃ : typeOf (Expr.call .durationSince xs) c₁ env = Except.ok (ty, c₂))
@@ -756,7 +756,7 @@ theorem type_of_call_durationSince_is_sound {xs : List Expr} {c₁ c₂ : Capabi
       simp only [Except.error.injEq, reduceCtorEq, or_self, or_false, or_true, true_and]
       apply type_is_inhabited_ext
 
-theorem type_of_call_ipAddr_recognizer_inversion {xfn : ExtFun} {xs : List Expr} {c c' : Capabilities} {env : Environment} {ty : TypedExpr}
+theorem type_of_call_ipAddr_recognizer_inversion {xfn : ExtFun} {xs : List Expr} {c c' : Capabilities} {env : TypeEnv} {ty : TypedExpr}
   (h₀ : IsIpAddrRecognizer xfn)
   (h₁ : typeOf (Expr.call xfn xs) c env = Except.ok (ty, c')) :
   ty.typeOf = .bool .anyBool ∧
@@ -788,7 +788,7 @@ theorem type_of_call_ipAddr_recognizer_inversion {xfn : ExtFun} {xs : List Expr}
     }
   }
 
-theorem type_of_call_ipAddr_recognizer_is_sound {xfn : ExtFun} {xs : List Expr} {c₁ c₂ : Capabilities} {env : Environment} {ty : TypedExpr} {request : Request} {entities : Entities}
+theorem type_of_call_ipAddr_recognizer_is_sound {xfn : ExtFun} {xs : List Expr} {c₁ c₂ : Capabilities} {env : TypeEnv} {ty : TypedExpr} {request : Request} {entities : Entities}
   (h₀ : IsIpAddrRecognizer xfn)
   (h₁ : CapabilitiesInvariant c₁ request entities)
   (h₂ : InstanceOfWellFormedEnvironment request entities env)
@@ -829,7 +829,7 @@ def IsDurationConverter : ExtFun → Prop
   | .toDays => True
   | _       => False
 
-theorem type_of_call_duration_converter_inversion {xfn : ExtFun} {xs : List Expr} {c c' : Capabilities} {env : Environment} {ty : TypedExpr}
+theorem type_of_call_duration_converter_inversion {xfn : ExtFun} {xs : List Expr} {c c' : Capabilities} {env : TypeEnv} {ty : TypedExpr}
   (h₀ : IsDurationConverter xfn)
   (h₁ : typeOf (Expr.call xfn xs) c env = Except.ok (ty, c')) :
   ty.typeOf = .int ∧
@@ -861,7 +861,7 @@ theorem type_of_call_duration_converter_inversion {xfn : ExtFun} {xs : List Expr
     }
   }
 
-theorem type_of_call_duration_converter_is_sound {xfn : ExtFun} {xs : List Expr} {c₁ c₂ : Capabilities} {env : Environment} {ty : TypedExpr} {request : Request} {entities : Entities}
+theorem type_of_call_duration_converter_is_sound {xfn : ExtFun} {xs : List Expr} {c₁ c₂ : Capabilities} {env : TypeEnv} {ty : TypedExpr} {request : Request} {entities : Entities}
   (h₀ : IsDurationConverter xfn)
   (h₁ : CapabilitiesInvariant c₁ request entities)
   (h₂ : InstanceOfWellFormedEnvironment request entities env)
@@ -894,7 +894,7 @@ theorem type_of_call_duration_converter_is_sound {xfn : ExtFun} {xs : List Expr}
     apply InstanceOfType.instance_of_int
   }
 
-theorem type_of_call_is_sound {xfn : ExtFun} {xs : List Expr} {c₁ c₂ : Capabilities} {env : Environment} {ty : TypedExpr} {request : Request} {entities : Entities}
+theorem type_of_call_is_sound {xfn : ExtFun} {xs : List Expr} {c₁ c₂ : Capabilities} {env : TypeEnv} {ty : TypedExpr} {request : Request} {entities : Entities}
   (h₁ : CapabilitiesInvariant c₁ request entities)
   (h₂ : InstanceOfWellFormedEnvironment request entities env)
   (h₃ : typeOf (Expr.call xfn xs) c₁ env = Except.ok (ty, c₂))
