cedar-lean/Cedar/Thm/Validation/Typechecker/IfThenElse.lean
@@ -25,7 +25,7 @@ namespace Cedar.Thm
 open Cedar.Spec
 open Cedar.Validation
 
-theorem type_of_ite_inversion {x₁ x₂ x₃ : Expr} {c c' : Capabilities} {env : Environment} {tx : TypedExpr}
+theorem type_of_ite_inversion {x₁ x₂ x₃ : Expr} {c c' : Capabilities} {env : TypeEnv} {tx : TypedExpr}
   (h₁ : typeOf (Expr.ite x₁ x₂ x₃) c env = Except.ok (tx, c')) :
   ∃ tx₁ bty₁ c₁ tx₂ c₂ tx₃ c₃,
     tx = TypedExpr.ite tx₁ tx₂ tx₃ tx.typeOf ∧
@@ -81,7 +81,7 @@ theorem type_of_ite_inversion {x₁ x₂ x₃ : Expr} {c c' : Capabilities} {env
     simp [TypedExpr.typeOf]
     exists res₃.snd
 
-theorem type_of_ite_is_sound {x₁ x₂ x₃ : Expr} {c₁ c₂ : Capabilities} {env : Environment} {ty : TypedExpr} {request : Request} {entities : Entities}
+theorem type_of_ite_is_sound {x₁ x₂ x₃ : Expr} {c₁ c₂ : Capabilities} {env : TypeEnv} {ty : TypedExpr} {request : Request} {entities : Entities}
   (h₁ : CapabilitiesInvariant c₁ request entities)
   (h₂ : InstanceOfWellFormedEnvironment request entities env)
   (h₃ : typeOf (Expr.ite x₁ x₂ x₃) c₁ env = Except.ok (ty, c₂))
