cedar-lean/Cedar/Thm/Validation/Typechecker/Or.lean
@@ -26,7 +26,7 @@ open Cedar.Data
 open Cedar.Spec
 open Cedar.Validation
 
-theorem type_of_or_inversion {x₁ x₂ : Expr} {c c' : Capabilities} {env : Environment} {tx : TypedExpr}
+theorem type_of_or_inversion {x₁ x₂ : Expr} {c c' : Capabilities} {env : TypeEnv} {tx : TypedExpr}
   (h₁ : typeOf (Expr.or x₁ x₂) c env = Except.ok (tx, c')) :
   ∃ tx₁ bty₁ c₁,
     typeOf x₁ c env = .ok (tx₁, c₁) ∧
@@ -96,7 +96,7 @@ theorem type_of_or_inversion {x₁ x₂ : Expr} {c c' : Capabilities} {env : Env
         specialize hneq₂ heq
         contradiction
 
-theorem type_of_or_is_sound {x₁ x₂ : Expr} {c₁ c₂ : Capabilities} {env : Environment} {ty : TypedExpr} {request : Request} {entities : Entities}
+theorem type_of_or_is_sound {x₁ x₂ : Expr} {c₁ c₂ : Capabilities} {env : TypeEnv} {ty : TypedExpr} {request : Request} {entities : Entities}
   (h₁ : CapabilitiesInvariant c₁ request entities)
   (h₂ : InstanceOfWellFormedEnvironment request entities env)
   (h₃ : typeOf (Expr.or x₁ x₂) c₁ env = Except.ok (ty, c₂))
