cedar-lean/Cedar/Thm/Validation/Validator.lean
@@ -39,7 +39,7 @@ def InstanceOfWellFormedSchema (schema : Schema) (request : Request) (entities :
   ∃ env ∈ schema.environments,
   InstanceOfWellFormedEnvironment request entities env
 
-theorem action_matches_env {env : Environment} {request : Request} {entities : Entities} :
+theorem action_matches_env {env : TypeEnv} {request : Request} {entities : Entities} :
   InstanceOfWellFormedEnvironment request entities env →
   request.action = env.reqty.action
 := by
@@ -48,7 +48,7 @@ theorem action_matches_env {env : Environment} {request : Request} {entities : E
   obtain ⟨_, ⟨ _, h₁, _, _ ⟩, _⟩ := h₀
   exact h₁
 
-theorem typecheck_policy_is_sound (policy : Policy) (env : Environment) (tx : TypedExpr) (request : Request) (entities : Entities) :
+theorem typecheck_policy_is_sound (policy : Policy) (env : TypeEnv) (tx : TypedExpr) (request : Request) (entities : Entities) :
   InstanceOfWellFormedEnvironment request entities env →
   typecheckPolicy policy env = .ok tx →
   ∃ b : Bool, EvaluatesTo policy.toExpr request entities b
@@ -67,7 +67,7 @@ theorem typecheck_policy_is_sound (policy : Policy) (env : Environment) (tx : Ty
   rw [←substitute_action_preserves_evaluates_to, action_matches_env h₁]
   exact h₄
 
-theorem typecheck_policy_with_environments_is_sound (policy : Policy) (envs : List Environment) (request : Request) (entities : Entities) :
+theorem typecheck_policy_with_environments_is_sound (policy : Policy) (envs : List TypeEnv) (request : Request) (entities : Entities) :
   (∃ env ∈ envs, InstanceOfWellFormedEnvironment request entities env) →
   typecheckPolicyWithEnvironments policy envs = .ok () →
   ∃ b : Bool, EvaluatesTo policy.toExpr request entities b
